%!TEX root = ../DDE-Project-Master.tex

\section{Uniform Convergence of Galerkin Solutions: System of DDEs case} \label{Sect_convergence_system_case}

\subsection{Multidimensional Case with Single Linear Delay Term}\label{section:single-linear-delay}

One can show that a similar convergence result holds for Galerkin approximations of 
\be
    \frac{\d \boldsymbol{x}(t)}{\d t}  = \boldsymbol{ Ax}(t)  + \boldsymbol {Bx}(t-\tau_p) + \boldsymbol{F} \left(\boldsymbol{x}(t-\tau_1), \cdots, \boldsymbol{x}(t-\tau_p)\right),
\ee
where \(\boldsymbol x(t)\) is a function from \([-\tau_p,\infty)\) to \(\mathbb R^d\) and \(\boldsymbol{F}:\mathbb R^{dp}\to \mathbb R^d\) is Lipschitz continuous. Instead of using \(\mcK_n^\tau\), we use the \(d\)-dimensional versions \(\mathbb K^\tau_n\) as introduced in \cite[Section~3.3]{CGLW16}. The results in \cref{prop:uniform-conv}, \cref{eq:uniform-bdd}, and \cref{eq:pw-conv} hold in appropriate ways for \(\mathbb K_n^\tau\) and can be proven using the one-dimensional case. Then the uniform convergence of the Galerkin approximations can be proven in an analogous way to \cref{thm:uniform_conv}. Namely, we introduce the inner product space
\be
    X_p := C^{+}([-\tau_p, 0);\mathbb R^d) \times \mathbb R^d
\ee
with the inner product 
\be
    (\Phi, \Psi)_{X_p} := (\Phi^S,\Psi^S)_{\R^d} + \frac 1 \tau (\Phi^D, \Psi^D)_{L^2([-\tau, 0) ; \R^d)} + \sum_{i=1}^p(\Phi^D(-\tau_i),\Psi^D(-\tau_i))_{\R^d}, \quad \Phi,\Psi\in X_p.
\ee
The above proofs can be edited to compensate for this new inner product. For instance, the line \cref{eq:pwx-1} would instead become
\bea
    \|T_N(t-s)\Pi_N(\mathcal F(u(s)) - \mathcal F(u_N(s)))\|_{X_p}^2 &= \|T_N(t-s)\Pi_N(\mathcal F(u(s)) - \mathcal F(u_N(s)))\|_\mcH^2 \\ 
    &+ \sum_{i=1}^p\left|[T_N(t-s)\Pi_N(\mathcal F(u(s)) - \mathcal F(u_N(s)))]^D(-\tau_i)\right|^2,
\eea
where we bound each \(\left|[T_N(t-s)\Pi_N(\mathcal F(u(s)) - \mathcal F(u_N(s)))]^D(-\tau_i)\right|\) in a similar way to how the single delay term was bounded.

\subsection{One Dimensional Case with Multiple Linear Delay Terms}\label{section:multiple-linear-delays}

We now consider the following one-dimensional DDE given by
\bea
    \frac{\d x(t)}{\d t} &= ax(t) + \sum_{i=1}^p b_i x(t-\tau_i) + F(x(t-\tau_1), x(t-\tau_2), \ldots, x(t-\tau_p)), \quad t > 0\\
    x(0) &= \alpha,  \\
    x(t) &= \varphi(t), \quad t\in [-\tau_p, 0)
\eea
where \(x(t)\) is a function from \([-\tau_p, \infty)\) to \(\R\) and \(F:\R^p\to\R\) is Lipschitz continuous. We embed this into the following multidimensional problem:
\bea
    \frac{\d\boldsymbol{ x}(t)}{\d t} &= \A \boldsymbol{x}(t) +   \B\,\begin{bmatrix}x_1(t-\tau_1) \\ x_2(t-\tau_2) \\ \vdots \\ x_p(t-\tau_p) \end{bmatrix} + \boldsymbol{F}(\boldsymbol x_t), & t&>0\\
    \boldsymbol{x}(0) &= [\alpha, \alpha, \cdots, \alpha]^T, \\
    x_1(\theta) &= \varphi(\theta), & -\tau_1\leq \theta&<0 \\
    x_2(\theta) &= \varphi(\theta), &  -\tau_2\leq \theta&<0 \\
    &\ \,  \vdots \\
    x_p (\theta) &= \varphi(\theta), &  -\tau_p\leq \theta&<0
\eea
where \(\A = a \boldsymbol{I}\) with \(\boldsymbol{I}\) the identity matrix, \(\B = \begin{bmatrix}1 & \cdots & 1\end{bmatrix}^T\begin{bmatrix}b_1 & \cdots & b_p\end{bmatrix}\), 
\be
    \boldsymbol F(\x_t) = \begin{bmatrix}F(x_1(t-\tau_1),\, x_2(t-\tau_2),\, \ldots,\, x_p(t-\tau_p)) \\ \vdots \\ F(x_1(t-\tau_1),\, x_2(t-\tau_2),\, \ldots,\, x_p(t-\tau_p))\end{bmatrix},
\ee
and \(x_i\) the \(i\)th component of \(\boldsymbol{x}\). Note that any \(x_i\) will satisfy the one-dimensional problem. Denote \(\boldtau = (\tau_1, \tau_2,\cdots,\tau_p)\). We may reference 
\be
    \begin{bmatrix}x_1(t-\tau_1) & x_2(t-\tau_2) & \cdots & x_p(t-\tau_p) \end{bmatrix}^T
\ee
by an abuse of notation, \(\boldsymbol{x}(t-\boldtau)\). We will prove results for the more general DDE given by
\bea\label{eq:multiple-delay-dde}
    \frac{\d\x(t)}{\d t} &= \A \boldsymbol{x}(t) +   \B\x(t-\boldtau) + \boldsymbol{G}(\x(t-\tau_1),\cdots,\x(t-\tau_p)), & t&>0\\
    \boldsymbol{x}(0) &= \boldgamma, \\
    x_1(\theta) &= f_1(\theta), & -\tau_1\leq \theta&<0 \\
    x_2(\theta) &= f_2(\theta), &  -\tau_2\leq \theta&<0 \\
    &\ \,  \vdots \\
    x_p (\theta) &= f_p(\theta), &  -\tau_p\leq \theta&<0
\eea
where \(\A, \B\in\mathbb R^{p\times p}\), \(\boldsymbol{G}:\R^p\to\R^p\) nonlinear, \(\boldgamma\in\R^p\) and \(f_i\in L^2([-\tau_i, 0);\mathbb R).\) Namely, we shall show that we can approximate the solution of the above by Galerkin problems using vectorized Koornwinder polynomials as defined in \cref{section:vectorized-koornwinder}. We can reformulate the above DDE to be in the form of an abstract Cauchy problem on \(\mcH^{\boldtau}\), which was defined in \cref{section:vectorized-koornwinder}. We define the linear operator \(\mcA: \mathcal D(\mcA) \to \mcH^{\boldtau}\) by 
\be\label{eq:multiple-delay-generator}
    \mcA\left(\begin{array} c \Psi^D \\  \Psi^S\end{array} \right):= \left(\begin{array} c \frac{d^+\Psi^D}{d\theta} \\ \boldsymbol A\Psi^S +  \boldsymbol B\Psi^D(-\boldtau)\end{array}\right)
\ee
with the domain of \(\mcA\) given by 
\be\label{eq:multiple-delay-domain}
    \mathcal D(\mcA) = \{(\Psi^D, \Psi^S)\in \mcH^{\boldtau}\, :\, \Psi_i^D\in H^1([-\tau_i, 0);\mathbb R),\, \lim_{\theta\to0^-} \Psi^D_i(\theta) = \Psi_i^S,\, \mbox{ for } i=1,\cdots, p\}.
\ee
The abstract ODE is then given by
\be\label{eq:abstract-ode-multiple-delay-case}
    \frac{\d u}{\d t} = \mcA u(t) + \mathcal G(u(t)),
\ee
with 
\bea \label{mcG}
    [\mcG (\Psi) ](\theta) & := \begin{cases}
    0, &  \theta \in[-\tau, 0),   \vspace{0.4em}\\ 
    \boldsymbol{G} \left( \Psi^D(-\tau) \right), & \theta = 0, 
    \end{cases}  \quad {\Forall \Psi = (\Psi^D, \Psi^S) \in  X_p}.
\eea
We also define the subspace 
\be\label{nspace}
    \mcH_N^{\boldtau} := \mathrm{span}\{\mathbb K^{\boldtau}_1, \cdots, \mathbb K^{\boldtau}_{Np}\},
\ee
i.e., it is the subspace of vectorized Koornwinder polynomials with degree less than or equal to \(N\). To get the \(Np\)-dimensional Galerkin approximation, we define the following operator
\be\label{GalOp}
    \mcA_N := \Pi_N\mcA\Pi_N,
\ee
where 
\be
    \Pi_N: \mcH^{\boldtau} \to \mcH_N^{\boldtau}
\ee
is the orthogonal projector into \(\mcH^{\boldtau}_N\). Note that \(\mathbb K^\tau_j\in\mathcal D(\mcA )\) for each \(j\in\mathbb N\), so \(\mcH^{\boldtau}_N\subset\mathcal D(\mcA)\) and the operator in \eqref{GalOp} is well-defined. We have the Galerkin problem given by
\be\label{eq:galerkin-multiple-delay-case}
     \frac{\d u_N}{\d t} = \mcA_N u_N(t) + \Pi_N\mcG(u_N(t)).
\ee
We can extend \(e^{\mcA_N t}\) to a \(C_0\)-semigroup \(T_N(t)\) on \(\mcH\) as follows:
\be
    T_N(t)u = e^{\mcA_N t}\Pi_Nu + (I-\Pi_N)u, \qquad u\in\mcH.
\ee
To apply the results given in \cite[Thm.~4.1]{CGLW16}, we need to prove the necessary assumptions about \(\mcA\) and \(\mcA_N\). That is, \(\mcA\) generates a \(C_0\) semigroup \(T(t)\) and
\ben[label= \textbf{(A\arabic*)}]
\item The following uniform bound is satisfied by \(\{T_N(t)\}_{N\geq0, t\geq 0}\)
\be
    \| T_N(t) \| \leq Me^{\omega t}, \qquad N\geq 0, \qquad t\geq 0
\ee
where \(\| T_N(t) \| = \sup\{ \| T_N(t) u \|_{\mcH^{\boldtau}} \mid  \|u\|_{\mcH^{\boldtau}} = 1, u \in \mcH^{\boldtau} \}\).
\item The following convergence holds:
\be
    \lim_{N\to\infty} \| \mcA_N u - \mcA u \|_{\mcH^{\boldtau}} = u, \qquad \forall u\in\mcH^{\boldtau}.
\ee
\een 
We first show that \(\mcA\) is an infinitesimal generator of a \(C_0\) semigroup. The proof will be similar to \cite[Thm 2.4.6]{CZ95}. We have the following result by slightly altering the proof from \cite[Thm 2.4.1]{CZ95}:

\bt
Consider the DDE \cref{eq:multiple-delay-dde}. For every \(\boldsymbol{\gamma}\in\mathbb R^p\) and for any choices of \(f_i\in L^2([-\tau_i,0);\mathbb R)\) for each \(i=1,2,\cdots, p\),  there exists a unique function \( \boldsymbol{x}(\cdot)\) on \([0,\infty)\) that is absolutely continuous and satisfies \cref{eq:multiple-delay-dde} almost everywhere. This function is called the solution of \cref{eq:multiple-delay-dde}, and it satisfies 
\be\label{eq:soln}
    \x(t) = e^{\A t} {\boldgamma}+ \int_0^t e^{\A(t-s)}\boldsymbol{Bx}(s-\boldtau)\, \d s \qquad \mbox{for } t\geq 0.
\ee
\et

We shall show that the following holds: 
\begin{lem}
If \( x(t)\) is the solution to \cref{eq:multiple-delay-dde}, then the following inequalities hold: 
\be\label{eq:ineq-Ct}
    |\boldsymbol{x}(t)|^2 \leq C_t\left[ |\boldsymbol\gamma|^2 + \sum_{i=1}^p\frac 1 {\tau_i}\|f_i\|^2_{L^2([-\tau_i,0);\mathbb R)}\right]
\ee
and 
\be\label{eq:ineq-Dt}
    \int_0^t |\boldsymbol{x}(s)|^2\, \d s \leq D_t\left[ |\boldsymbol{\gamma}|^2 + \sum_{i=1}^p\frac 1 {\tau_i}\|f_i\|^2_{L^2([-\tau_i,0);\mathbb R)}\right],
\ee
where \(C_t\) and \(D_t\) are constants  that depend only on \(t\). 
\end{lem}

\begin{proof}
We know that for \(e^{\A t}\) there exists \(M_0>0\) and \(\omega>0\) such that \(|e^{\A t}|\leq M_0e^{\omega t}\). Let \[M:=\max\{M_0, |\B|\}.\] Then from \cref{eq:soln} we have
\bea\label{ineq1}
    | \x(t) | &\leq |\boldgamma||e^{\A t}| + \left|\int_0^t  e^{\A t}\B \x(s-\boldtau)\d s\right| \\
    &\leq M_0|\boldgamma|e^{\omega t} + \int_0^t M_0e^{\omega(t-s)}| \B||\x(s-\boldtau)| \d s \\
    &\leq M|\boldgamma|e^{\omega t} + M^2\int_0^t e^{\omega(t-s)}|\x(s-\boldtau)| \d s \\
    &\leq M|\boldgamma|e^{\omega t} + M^2\sum_{i=1}^p\int_0^t e^{\omega(t-s)}|x_i(s-\tau_i)| \d s \\
    &= M|\boldgamma|e^{\omega t} + M^2e^{\omega t}\sum_{i=1}^p\int_{-\tau_i}^{t-\tau_i} e^{-\omega(\theta+\tau_i)}|x_i(\theta)| \d s. \\
\eea
We also have that for \(i=1,2,\cdots, p\)
\bea\label{ineq2}
    \int_{-\tau_i}^{t-\tau_i} e^{-\omega(\theta+\tau_i)}|x_i(\theta)|\,d\theta &\leq \int_{-\tau_i}^0e^{-\omega(\theta+\tau_i)}|x_i(\theta)|\,d\theta + \int_0^te^{-|a|(\theta+\tau_i)}|x_i(\theta)|\d\theta \\
    &= \int_{-\tau_i}^0e^{-\omega(\theta+\tau_i)}|f_i(\theta)|\,d\theta + \int_0^te^{-|a|(\theta+\tau_i)}| x_i(\theta)|\d\theta \\
    &\leq \int_{-\tau_i}^0|f_i(\theta)|\,d\theta + \int_0^te^{-\omega(\theta+\tau_i)}| x_i(\theta)|\d\theta \\
    &\leq \sqrt{\tau_i} \|f_i\|_{L^2([-\tau_i, 0);\mathbb R)} +  \int_0^te^{-\omega(\theta+\tau_i)}| x_i(\theta)|\d\theta \\
    &\leq \sqrt{\tau_i} \|f_i\|_{L^2([-\tau_i, 0);\mathbb R)} +  \int_0^te^{-\omega\theta}| x_i(\theta)|\d\theta \\
    &\leq \sqrt{\tau_i} \|f_i\|_{L^2([-\tau_i, 0);\mathbb R)} +  \int_0^te^{-\omega\theta}| x_i(\theta)|\d\theta.
\eea
From \eqref{ineq1} and \eqref{ineq2} we have 

\bea
    | \x(t) | &\leq M|\boldgamma|e^{\omega t} + M^2e^{\omega t}\sum_{i=1}^p\left[\sqrt{\tau_i} \|f_i\|_{L^2([-\tau_i, 0);\mathbb R)} +  \int_0^te^{-\omega\theta}| \x(\theta)|\d\theta \right] \\
    &\leq M|\boldgamma|e^{\omega t} + M^2e^{\omega t}\sum_{i=1}^p\left[\sqrt{\tau_i} \|f_i\|_{L^2([-\tau_i, 0);\mathbb R)} \right]+  M^2e^{\omega t}p\int_0^te^{-\omega\theta}| \x(\theta)|\d\theta.
\eea
Set \(\alpha = M|\boldgamma| + M^2\sum_{i=1}^p\left[\sqrt{\tau_i} \|f_i\|_{L^2([-\tau_i, 0);\mathbb R)} \right]\), \(\beta = M^2p\) and \(g(t) = e^{-\omega t}| \x(t)|\), we get the following inequality
\be
    g(t) \leq \alpha + \beta\int_0^t g(\theta) \d\theta.
\ee
Applying the integral form of Gr\"onwall's inequality yields 
\be
    g(t) \leq \alpha e^{\beta t}. 
\ee
Thus 
\bea
    | \x(t) | &\leq e^{(M^2p + \omega)t}\left[ M|\boldgamma| + M^2\sum_{i=1}^p\sqrt{\tau_i} \|f_i\|_{L^2([-\tau_i, 0);\mathbb R)}\right] \\
    &\leq e^{(M^2p + \omega)t}\left[ M|\boldgamma| + M^2\tau_p\sum_{i=1}^p\frac 1 {\sqrt{\tau_i}} \|f_i\|_{L^2([-\tau_i, 0);\mathbb R)}\right] \\
    &\leq e^{(M^2p + \omega)t}\max\{M, M^2\tau_p\}\left[|\boldgamma| + \sum_{i=1}^p\frac 1 {\sqrt{\tau_i}} \|f_i\|_{L^2([-\tau_i, 0);\mathbb R)}\right] \\
\eea
and squaring both sides yields
\be
    | \x(t)|^2 \leq e^{2(M^2p + \omega)t}(\max\{M, M^2\tau_p\})^2\left[|\boldgamma|^2 + \sum_{i=1}^p\frac 1 {\tau_i} \|f_i\|^2_{L^2([-\tau_i, 0);\mathbb R)}\right].
\ee 
This gives \cref{eq:ineq-Ct}, and integrating gives \cref{eq:ineq-Dt}.
\end{proof}

The following theorems are proven similarly to \cite[Thm 2.4.4]{CZ95} and \cite[Thm 2.4.6]{CZ95}.
\bt
Let the operator \(T(t)\) be defined by
\be\label{operator}
    T(t)\left(\begin{array}{c} f(\cdot) \\ \boldgamma \end{array}\right) := \left(\begin{array} c \x(t+\cdot) \\ \x(t)\end{array}\right),
\ee
where \(\x(\cdot)\) is the solution to \cref{eq:multiple-delay-dde}. Then \(T(t)\) for \(t\geq 0\) satisfies:
\begin{enumerate}[label=\roman*.]
\item \(T(t)\in\mathcal L(\mcH^{\boldtau})\) for all \(t\geq 0\);
\item \(T(t)\) is a \(C_0-\)semigroup on \(\mcH^{\boldtau}\).
\end{enumerate}
\et

\bt
Consider the \(C_0\)-semigroup defined by \eqref{operator}. Its infinitesimal generator is given by \cref{eq:multiple-delay-generator} with domain \cref{eq:multiple-delay-domain}.
\et
The assumption given by \textbf{(A2)} is proven nearly identically to \cite[Lem.~4.1]{CGLW16}. The assumption \textbf{(A3)} requires more details but follows a similar argument to those given in \cite[Lem.~4.2, Lem.~4.3]{CGLW16}.
\bprop
Let \(\mcA\) be defined such as in \cref{eq:multiple-delay-generator}. Then 
\be
    \iph {\mcA\Psi} {\Psi} \leq \omega\|\Psi\|^2_{\mcH^{\boldtau}}, \quad \forall\Psi\in\mathcal D(\mcA),
\ee
with 
\be\label{eq:omega}
    \omega = \left(\frac 1 {2\tau_1} + |\A| + \frac{\tau_p} 2 |\B|^2\right).
\ee
\eprop

\bp
Let \(\Psi\in\mathcal D(\mcA)\). By the definition of \(\mcA\), we have
\be
    \iph {\mcA \Psi} {\Psi} = \underbrace{\sum_{i=1}^p \frac 1 {\tau_i} \int_{-\tau_i}^0 \frac{\d^+\Psi_i^D}{\d\theta}(\theta)\Psi_i^D(\theta)\d\theta}_\text{(1)} + \underbrace{\ip {\A\Psi^S} {\Psi^S} }_\text{(2)}+ \underbrace{\ip {\B\Psi^D(-\tau)}{\Psi^S}}_\text{(3)}.
\ee
\ben[label=(\arabic*)]
\item For \(i=1,2,\ldots, p\), we have 
\bea
    \frac 1 {\tau_i} \int_{-\tau_i}^0 \frac{\d^+\Psi_i^D}{\d\theta}(\theta)\Psi_i^D(\theta)\d\theta &= \frac 1 {2\tau_i}\left((\Psi_i^S)^2 - (\Psi^D_i(-\tau_i))^2 \right) \\
    &\leq \frac 1 {2\tau_1}(\Psi_i^S)^2 - \frac 1 {2\tau_p}(\Psi_i^D(-\tau_i))^2.
\eea
So 
\be
    \sum_{i=1}^p\frac 1 {\tau_i} \int_{-\tau_i}^0 \frac{\d^+\Psi_i^D}{\d\theta}(\theta)\Psi_i^D(\theta)\d\theta \leq \frac 1 {\tau_1} |\Psi^S|^2 - \frac 1 {2\tau_p}|\Psi^D(-\tau)|^2.
\ee
\item We have 
\be
    \ip {\A\Psi^S} {\Psi^S} \leq |\A||\Psi^S|^2.
\ee
\item We have 
\bea
    \ip{\B\Psi^D(-\tau)}{\Psi^S} &\leq |\B||\Psi^D(-\tau)||\Psi^S| \\
    &= \left(\frac 1 {\sqrt{\tau_p}} |\Psi^D(-\tau)|\right)\left(\sqrt{\tau_p} |\B| |\Psi^S|\right)\\
    &\leq \frac{|\Psi^D(-\tau)|^2}{2\tau_p} + \frac{\tau_p|\B|^2|\Psi^S|^2}{2}.
\eea
\een
Thus from (1), (2), and (3), we have that 
\bea
    \iph {\mcA \Psi} {\Psi} &=  \left(\frac 1 {2\tau_1} + |\A| + \frac{\tau_p}{2}|\B|^2 \right)|\Psi^S|^2 \\
    &\leq  \left(\frac 1 {2\tau_1} + |\A| + \frac{\tau_p}{2}|\B|^2 \right) \|\Psi\|^2_{\mcH^{\boldtau}},
\eea
as desired.
\ep


We now prove the following statement:

\bprop
Let  \(\mcA\) be defined as in \cref{eq:multiple-delay-generator}. Then, the linear semigroups $T(t)$ and $T_N(t)$ generated respectively by \(\mcA\) and \(\mcA_N\)  defined in \eqref{GalOp},  satisfy 
\be\label{stable_estimates}
    \|T(t)\| \le e^{\omega t} \quad \text{ and }  \quad \|T_N(t)\| \le e^{\omega t}, \qquad t \ge 0,
\ee
with \(\omega\) given by \cref{eq:omega}.
\eprop

\bp
We have that \(T(t)\) is a \(C_0\)-semigroup with infinitesimal generator \(\mcA\). By \cite[Thm. 2.4 c) p.5]{P83}, it follows that \(T(t)u_0\in \mathcal D(\mcA)\) for all \(u_0\in\mathcal D(\mcA)\) and that 
\be
    \frac{\d}{\d t} T(t)u_0 = \mathcal{A} T(t) u_0,   \qquad \Forall u_0 \in \mathcal{A}, \; t \ge 0.
\ee

Thus 
\bea
    \frac \d {\d t} \|T(t) u_0\|^2_{\mcH^{\boldtau}} &= 2\iph{\mcA T(t)u_0}{T(t)u_0} \\
    &\leq 2\omega\|T(t)u_0\|^2_{\mcH^{\boldtau}},
\eea
for any \(u_0\in\mathcal D(\mcA).\) Applying Gronwall's inequality and taking the square root of both sides gives
\be
    \|T(t)u_0\|_{\mcH}\leq  e^{\omega t} \|u_0\|_{\mcH},
\ee
for \(u_0\in\mathcal D(\mcA).\) For \(x\in\mcH\), since \(\mathcal D(\mcA)\) is dense in \(\mcH\) we can pick \(\{u_n\}_{n=1}^\infty\subset \mathcal D(\mcA)\) where \(u_n\to x\) in \(\mcH^{\boldtau}\). Thus
\bea
    \|T(t)x\|_{\mcH^{\boldtau}} &= \|T(t)(x-u_n+u_n)\|_{\mcH^{\boldtau}} \\
    &\leq \|T(t)\|_{\mcH^{\boldtau}}\cdot \|x-u_n\|_{\mcH^{\boldtau}} + e^{\omega t} \|u_n\|_{\mcH^{\boldtau}},
\eea
where the first term on the right goes to \(0\) and the second term on the right goes to \(e^{\omega t}\|x\|_{\mcH}\) as \(n\to\infty\). Thus the inequality holds for all \(x\in \mcH\) and 
\be
    \|T(t)\|_{\mcH^{\boldtau}} \leq e^{\omega t}, \qquad t\geq 0.
\ee
For the estimate on \(T_N\), we first note that for \(u_0\in\mcH\)
\bea
    \|T_N(t) u_0\|^2_{\mcH^{\boldtau}} & = \big\langle e^{\mathcal{A}_N t} \Pi_N u_0 + (I - \Pi_N) u_0, e^{\mathcal{A}_N t} \Pi_N u_0 + (I - \Pi_N) u_0 \big\rangle_{\mcH^{\boldtau}} \\
    & = \big\langle e^{\mcA_N t} \Pi_N u_0, e^{\mathcal{A}_N t} \Pi_N u_0  \big\rangle_{\mcH^{\boldtau}} + \big\langle (I - \Pi_N) u_0, (I - \Pi_N) u_0  \big\rangle_{\mcH^{\boldtau}} \\
    & = \| e^{\mathcal{A}_N t} \Pi_N u_0 \|^2_{\mcH^{\boldtau}} + \| (I - \Pi_N) u_0\|^2_{\mcH^{\boldtau}}.
\eea
Also note for \(\varphi,\psi\in\mcH^{\boldtau}\) that
\bea
    \iph{\Pi_N\varphi}{\psi} &= \iph{\varphi}{\Pi_N\psi} - \iph{(I-\Pi_N)\varphi}{\Pi_N\psi} + \iph{\Pi_N\varphi}{(I-\Pi_N)\psi} \\
    &=\iph{\varphi}{\Pi_N\psi},
\eea
where \((I-\Pi_N)\varphi\) and \((I-\Pi_N)\psi\) are orthogonal to the space \(\mcH_N\) and the terms \(\iph{(I-\Pi_N)\varphi}{\Pi_N\psi}\) and \(\iph{\Pi_N\varphi}{(I-\Pi_N)\psi}\) evaluate to \(0\). We can thus justify moving \(\Pi_N\) between terms in \(\iph \cdot\cdot.\) Therefore
\bea
    \frac\d{\d t} \|T_N(t) u_0\|^2_{\mcH^{\boldtau}} &= \frac\d{\d t}\| e^{\mathcal{A}_N t} \Pi_N u_0 \|^2_{\mcH^{\boldtau}} \\
    &= 2\iph{\mcA_Ne^{\mcA_Nt}\Pi_N u_0}{e^{\mcA_Nt}\Pi_N u_0} \\
    &= 2\iph{\Pi_N\mcA\Pi_Ne^{\mcA_Nt}\Pi_N u_0}{e^{\mcA_Nt}\Pi_N u_0} \\
    &= 2\iph{\mcA\Pi_Ne^{\mcA_Nt}\Pi_N u_0}{\Pi_Ne^{\mcA_Nt}\Pi_N u_0} \\
    &\leq 2\omega\|e^{\mcA_Nt}\Pi_N u_0\|_{\mcH^{\boldtau}}^2 \\
    &\leq 2\omega\left(\|e^{\mcA_Nt}\Pi_N u_0\|_{\mcH^{\boldtau}}^2 + \|(I - \Pi_N) u_0\|^2_{\mcH^{\boldtau}} \right) \\
    &= \|T_N(t) u_0\|^2_{\mcH^{\boldtau}}
\eea
Again applying Gronwall's inequality and taking the square root of each side gives 
\be
    \|T(t)u_0\|_{\mcH^{\boldtau}} \leq e^{\omega t} \|u_0\|_{\mcH^{\boldtau}}, \qquad u_0\in\mcH^{\boldtau},
\ee
which implies the desired inequality.
\ep

Thus we have \textbf{(A2)}. We can now apply the results of \cite[Thm.~4.1]{CGLW16}. A similar argument as given \cref{section:single-linear-delay} allows us to extend the arguments given in \cref{section:convergence} of this paper and control the term \(\mcG\) appropriately. If \(u\) and \(u_N\) are solutions to \cref{eq:abstract-ode-multiple-delay-case} and \cref{eq:galerkin-multiple-delay-case} respectively, we have that 
\be
    \lim_{N\to\infty} \sup_{t\in[0,T]}\| u(t) - u_N(t) \|_{\mcH^{\boldtau}} = 0.
\ee

\subsection{Multidimensional Case with Multiple Linear Delay Terms}

We now consider the \(d\)-dimensional DDE of the form:
\be
    \frac{\d \x(t)}{\d t}  = \A \x(t)  + \sum_{i=1}^p \B_i  \x(t-\tau_i) +  \boldsymbol{F} (\x(t-\tau_1), \cdots, \x(t-\tau_p)).
\ee
We can imbed this into a \((d\times p)\)-dimensional problem given by
\be
    \begin{bmatrix}\dot{\x}_1(t) \\ \dot{\x}_2(t) \\ \vdots \\ \dot{\x}_p(t)\end{bmatrix} = \widetilde{\A}\begin{bmatrix}{\x}_1(t) \\ {\x}_2(t) \\ \vdots \\ {\x}_p(t)\end{bmatrix} + \widetilde{\B}\begin{bmatrix}{\x}_1(t-\tau_1) \\ {\x}_2(t-\tau_2) \\ \vdots \\ {\x}_p(t-\tau_p)\end{bmatrix} + \begin{bmatrix} \boldsymbol{F} (\x_1(t-\tau_1), \x(t-\tau_2), \cdots, \x_p(t-\tau_p)) \\ \boldsymbol{F} (\x_1(t-\tau_1), \x(t-\tau_2), \cdots, \x_p(t-\tau_p)) \\ \vdots \\ \boldsymbol{F} (\x_1(t-\tau_1), \x(t-\tau_2), \cdots, \x_p(t-\tau_p))\end{bmatrix},
\ee
where 
\be
    \widetilde{\A} := \begin{bmatrix}\A & & & \\ & \A & & \\ & & \ddots & \\ & & & \A \end{bmatrix} \hspace{2em} \mbox{ and }\hspace{2em} \widetilde{\B} := \begin{bmatrix}\B_1 & \B_2 & \cdots & \B_p \\ \B_1 & \B_2 & \cdots & \B_p \\ \vdots & \vdots & & \vdots \\ \B_1 & \B_2 & \cdots & \B_p\end{bmatrix}.
\ee
This problem is of the form given in \cref{eq:multiple-delay-dde}. We set 
\be
    \boldtau = (\underbrace{\tau_1, \cdots, \tau_1}_{\text{\(d\) times}}, \underbrace{\tau_2, \cdots, \tau_2}_{\text{\(d\) times}}, \cdots, \underbrace{\tau_p, \cdots, \tau_p}_{\text{\(d\) times}})\
\ee
and define a linear operator \(\mcA\) on the space \(\mcH^{\boldtau}\). As we have seen in \cref{section:multiple-linear-delays}, we can approximate the solution of this abstract ODE on \(\mcH^{\boldtau}\) via a Galerkin scheme.